PAC: uint64 should be machine words in generated code, not the default IntInf

PAC_Checker2/EPAC_Efficient_Checker_Synthesis.thy
@@ -2430,11 +2430,9 @@ where
     else do {
       PAC_checker_l_s spec' (\<V>, A) b st
      }
-      }\<close>
+   }\<close>
 
 sepref_register remap_polys_l2_with_err_s full_checker_l_s2 PAC_checker_l_s
-term PAC_checker_l_s
-thm PAC_checker_l_s_impl.refine
 
 sepref_definition full_checker_l_s2_impl
   is \<open>uncurry2 full_checker_l_s2\<close>
@@ -2456,8 +2454,117 @@ local_setup \<open>
 
 declare version_def [code]
 
+definition uint32_of_uint64 :: \<open>uint64 \<Rightarrow> uint32\<close> where
+  \<open>uint32_of_uint64 n = uint32_of_nat (nat_of_uint64 n)\<close>
+
+lemma [code]: \<open>hashcode n = uint32_of_uint64 (n AND 4294967295)\<close> for n :: uint64
+  unfolding hashcode_uint64_def uint32_of_uint64_def by auto
+
+(*TODO this is a copy paste because of the order of the merge *)
+code_printing code_module Uint64 \<rightharpoonup> (SML) \<open>(* Test that words can handle numbers between 0 and 63 *)
+val _ = if 6 <= Word.wordSize then () else raise (Fail ("wordSize less than 6"));
+
+structure Uint64 : sig
+  eqtype uint64;
+  val zero : uint64;
+  val one : uint64;
+  val fromInt : IntInf.int -> uint64;
+  val toInt : uint64 -> IntInf.int;
+  val toFixedInt : uint64 -> Int.int;
+  val toLarge : uint64 -> LargeWord.word;
+  val fromLarge : LargeWord.word -> uint64
+  val fromFixedInt : Int.int -> uint64
+  val toWord32: uint64 -> Word32.word
+  val plus : uint64 -> uint64 -> uint64;
+  val minus : uint64 -> uint64 -> uint64;
+  val times : uint64 -> uint64 -> uint64;
+  val divide : uint64 -> uint64 -> uint64;
+  val modulus : uint64 -> uint64 -> uint64;
+  val negate : uint64 -> uint64;
+  val less_eq : uint64 -> uint64 -> bool;
+  val less : uint64 -> uint64 -> bool;
+  val notb : uint64 -> uint64;
+  val andb : uint64 -> uint64 -> uint64;
+  val orb : uint64 -> uint64 -> uint64;
+  val xorb : uint64 -> uint64 -> uint64;
+  val shiftl : uint64 -> IntInf.int -> uint64;
+  val shiftr : uint64 -> IntInf.int -> uint64;
+  val shiftr_signed : uint64 -> IntInf.int -> uint64;
+  val set_bit : uint64 -> IntInf.int -> bool -> uint64;
+  val test_bit : uint64 -> IntInf.int -> bool;
+end = struct
+
+type uint64 = Word64.word;
+
+val zero = (0wx0 : uint64);
+
+val one = (0wx1 : uint64);
+
+fun fromInt x = Word64.fromLargeInt (IntInf.toLarge x);
+
+fun toInt x = IntInf.fromLarge (Word64.toLargeInt x);
+
+fun toFixedInt x = Word64.toInt x;
+
+fun fromLarge x = Word64.fromLarge x;
+
+fun fromFixedInt x = Word64.fromInt x;
+
+fun toLarge x = Word64.toLarge x;
+
+fun toWord32 x = Word32.fromLarge x
+
+fun plus x y = Word64.+(x, y);
+
+fun minus x y = Word64.-(x, y);
+
+fun negate x = Word64.~(x);
+
+fun times x y = Word64.*(x, y);
+
+fun divide x y = Word64.div(x, y);
+
+fun modulus x y = Word64.mod(x, y);
+
+fun less_eq x y = Word64.<=(x, y);
+
+fun less x y = Word64.<(x, y);
+
+fun set_bit x n b =
+  let val mask = Word64.<< (0wx1, Word.fromLargeInt (IntInf.toLarge n))
+  in if b then Word64.orb (x, mask)
+     else Word64.andb (x, Word64.notb mask)
+  end
+
+fun shiftl x n =
+  Word64.<< (x, Word.fromLargeInt (IntInf.toLarge n))
+
+fun shiftr x n =
+  Word64.>> (x, Word.fromLargeInt (IntInf.toLarge n))
+
+fun shiftr_signed x n =
+  Word64.~>> (x, Word.fromLargeInt (IntInf.toLarge n))
+
+fun test_bit x n =
+  Word64.andb (x, Word64.<< (0wx1, Word.fromLargeInt (IntInf.toLarge n))) <> Word64.fromInt 0
+
+val notb = Word64.notb
+
+fun andb x y = Word64.andb(x, y);
+
+fun orb x y = Word64.orb(x, y);
+
+fun xorb x y = Word64.xorb(x, y);
+
+end (*struct Uint64*)
+\<close>
+
 code_printing constant arl_get_u' \<rightharpoonup> (SML) "(fn/ ()/ =>/ Array.sub/ ((fn/ (a,b)/ =>/ a) ((_)),/ Word64.toInt (Uint64.toLarge ((_)))))"
-  thm PAC_checker_l_s_impl_def
+
+definition uint32_of_uint64' where
+  [symmetric, code]: "uint32_of_uint64' = uint32_of_uint64"
+code_printing constant uint32_of_uint64' \<rightharpoonup> (SML) "Uint64.toWord32 ((_))"
+
 export_code(*  PAC_update_impl PAC_empty_impl the_error is_cfailed is_cfound
    * int_of_integer Del CL nat_of_integer String.implode remap_polys_l2_with_err_s_impl
    * union_vars_poly_impl empty_vars_impl PAC_checker_l_step_s_impl
